libcrux-ml-kem/proofs/fstar/spec/Spec.MLKEM.Math.fst
@@ -194,6 +194,7 @@ let compute_As_plus_e_ntt #p a s e = vector_add (matrix_vector_mul_ntt a s) e
 type dT = d: nat {d = 1 \/ d = 4 \/ d = 5 \/ d = 10 \/ d = 11 \/ d = 12}
 let max_d (d:dT) = if d < 12 then pow2 d else v v_FIELD_MODULUS
 type field_element_d (d:dT) = n:nat{n < max_d d}
+
 type polynomial_d (d:dT) = t_Array (field_element_d d) (sz 256)
 type vector_d (r:rank) (d:dT) = t_Array (polynomial_d d) r
 
@@ -228,11 +229,25 @@ let decompress_d (d: dT {d <> 12}) (x: field_element_d d): field_element
   = let r = (x * v v_FIELD_MODULUS + 1664) / pow2 d in
     r
     
-
 let byte_encode (d: dT) (coefficients: polynomial_d d): t_Array u8 (sz (32 * d))
   =  let coefficients' : t_Array nat (sz 256) = map_array #(field_element_d d) (fun x -> x <: nat) coefficients in
      bits_to_bytes #(sz (32 * d))
        (retype_bit_vector (bit_vec_of_nat_array coefficients' d))
+
+let serialize_post
+  (d: dT)
+  (coefficients: polynomial {
+    forall i. i < d * 
+  })
+  (output: t_Array u8 (sz (2 * d)))
+  = coefficients
+
+// let byte_encode' 
+//   (d: dT)
+//   #t
+//   (coefficients:  {forall i. bounded (Seq.index coefficients i) d})
+//   : t_Array u8 (sz (32 * d))
+//   = admit ()
 
 let byte_decode (d: dT) (coefficients: t_Array u8 (sz (32 * d))): polynomial_d d
   = let bv = bytes_to_bits coefficients in
